theories/RTac/Fail.v
@@ -9,20 +9,16 @@ Set Strict Implicit.
 Section parameterized.
   Context {typ : Type}.
   Context {expr : Type}.
-  Context {subst : Type}.
 
   Context {RType_typ : RType typ}.
   Context {Expr_expr : Expr RType_typ expr}.
   Context {Typ0_Prop : Typ0 _ Prop}.
-  Context {Subst_subst : Subst subst expr}.
-  Context {SubstUpdate_subst : SubstUpdate subst expr}.
-  Context {SubstOk_subst : @SubstOk _ _ _ _ Expr_expr Subst_subst}.
 
-  Definition FAIL : rtac typ expr subst :=
+  Definition FAIL : rtac typ expr :=
     fun _ _ _ _ _ _ _ => Fail.
 
   Theorem FAIL_sound
-  : forall tus tvs, rtac_sound tus tvs FAIL.
+  : rtac_sound FAIL.
   Proof.
     unfold FAIL, rtac_sound.
     intros; subst.
