theories/RTac/RunOnGoals.v
@@ -29,163 +29,9 @@ Section runOnGoals.
   Context {Expr_expr : Expr RType_typ expr}.
   Context {Typ0_Prop : Typ0 _ Prop}.
 
-(*
-  Fixpoint forgets (from : nat) (ts : list typ) (s : FMapSubst.SUBST.raw expr)
-  : list (option expr) :=
-    match ts with
-      | nil => nil
-      | t :: ts =>
-        let rr := forgets (S from) ts s in
-        let ne := subst_lookup from s in
-        ne :: rr
-    end.
-
-  Fixpoint remembers (from : nat) (tes : list (typ * option expr)) (s : subst)
-  : option subst :=
-    match tes with
-      | nil => Some s
-      | (_,None) :: tes' => remembers (S from) tes' s
-      | (_,Some e) :: tes' =>
-        (* This should not be necessary but to eliminate it, we must have a
-         * syntactic soundness condition for [set] *)
-        match subst_lookup from s with
-          | None =>
-            match subst_set from e s with
-              | None => None
-              | Some s' => remembers (S from) tes' s'
-            end
-          | Some _ => None
-        end
-    end.
-*)
-
   Lemma iff_to_eq : forall P Q : Prop, P = Q -> (P <-> Q).
   Proof. clear; intros; subst; reflexivity. Qed.
 
-(*
-  Lemma remembers_spec
-  : forall l tus tvs s s' sD gsD,
-      WellFormed_subst s ->
-(*      (forall x, x >= length tus -> lookup x s = None) -> *)
-      remembers (length tus) l s = Some s' ->
-      substD (tus ++ map fst l) tvs s = Some sD ->
-      goal_substD tus tvs (map fst l) (map snd l) = Some gsD ->
-      exists s'D,
-        substD (tus ++ map fst l) tvs s' = Some s'D /\
-        forall us vs, (gsD us vs /\ sD us vs) <-> s'D us vs.
-  Proof.
-    induction l; simpl; intros.
-    { forward_reason; inv_all; subst.
-      eexists; split; eauto. intros. tauto. }
-    { forward_reason; inv_all; subst.
-      destruct a; simpl in *.
-      destruct o; forward; inv_all; subst.
-      { replace (S (length tus)) with (length (tus ++ t :: nil)) in H6
-          by (rewrite app_length; simpl; omega).
-        rewrite substD_conv with (pfu := app_ass_trans tus (t :: nil) (map fst l))
-                                   (pfv := eq_refl) in H1.
-        rewrite exprD'_conv with (pfu := app_ass_trans tus (t :: nil) (map fst l))
-                                   (pfv := eq_refl) in H2.
-        autorewrite with eq_rw in H1.
-        autorewrite with eq_rw in H2.
-        forward; inv_all; subst.
-        specialize (@IHl (tus ++ t :: nil) tvs).
-        eapply set_sound in H5; eauto. destruct H5.
-        assert (subst_lookup (length tus) s = None) by eauto.
-        specialize (fun x y => H5 H7 _ _ t _ x _ H1 y H2); clear H7.
-        assert (exists get,
-                  nth_error_get_hlist_nth typD ((tus ++ t :: nil) ++ map fst l)
-                                          (length tus) =
-                  Some
-                    (existT
-                       (fun t0 : typ =>
-                          hlist typD ((tus ++ t :: nil) ++ map fst l) -> typD t0) t get) /\
-                  forall us us',
-                    get (hlist_app us us') = hlist_get_cons_after_app us).
-        { clear.
-          induction tus; simpl.
-          { eexists; split; eauto.
-            unfold hlist_get_cons_after_app. simpl.
-            intros. rewrite (hlist_eta us). reflexivity. }
-          { destruct IHtus as [ ? [ ? ? ] ].
-            rewrite H. eexists; split; eauto.
-            intros. unfold hlist_get_cons_after_app.
-            simpl. rewrite (hlist_eta us). simpl.
-            rewrite H0.
-            unfold hlist_get_cons_after_app.
-            reflexivity. } }
-        destruct H7 as [ ? [ ? ? ] ].
-        eapply H5 in H7; clear H5.
-        forward_reason.
-        specialize (IHl _ _ _ _ H4 H6 H5 H3).
-        forward_reason.
-        rewrite substD_conv with (pfu := eq_sym (app_ass_trans tus (t :: nil) (map fst l)))
-                                   (pfv := eq_refl) in H10.
-        autorewrite with eq_rw in H10. simpl in *.
-        forward.
-        eexists; split; eauto.
-        inv_all; subst. intros.
-        autorewrite with eq_rw.
-        specialize (H11 (hlist_app (hlist_app (fst (hlist_split _ _ us))
-                                              (Hcons (hlist_hd (snd (hlist_split _ _ us))) Hnil))
-                                   (hlist_tl (snd (hlist_split _ _ us)))) vs).
-        specialize (H9 (hlist_app (hlist_app (fst (hlist_split _ _ us))
-                                              (Hcons (hlist_hd (snd (hlist_split _ _ us))) Hnil))
-                                   (hlist_tl (snd (hlist_split _ _ us)))) vs).
-        specialize (H8 (hlist_app (fst (hlist_split _ _ us))
-                                  (Hcons (hlist_hd (snd (hlist_split _ _ us))) Hnil))
-                                   (hlist_tl (snd (hlist_split _ _ us)))).
-        rewrite <- (hlist_app_hlist_split _ _ us).
-        revert H9. revert H8. revert H11.
-        clear. rewrite hlist_app_assoc.
-        simpl.
-        generalize dependent (app_ass_trans tus (t :: nil) (map fst l)).
-        generalize dependent (hlist_split tus (t :: map fst l) us).
-        clear.
-        generalize dependent ((tus ++ t :: nil) ++ map fst l).
-        intros; subst. simpl in *.
-        assert ((Hcons (hlist_hd (snd p)) (hlist_tl (snd p))) = snd p).
-        { rewrite (hlist_eta (snd p)). f_equal. }
-        rewrite H in *.
-        rewrite and_comm.
-        rewrite and_assoc. rewrite and_comm in H11.
-        rewrite <- H11; clear H11.
-        rewrite H8 in H9; clear H8.
-        rewrite H9; clear H9.
-        repeat rewrite <- and_assoc.
-        eapply and_iff. reflexivity.
-        intro. rewrite and_comm.
-        eapply and_iff; eauto.
-        { eapply iff_to_eq. f_equal. rewrite <- H. simpl.
-          clear.
-          generalize dependent (fst p).
-          generalize dependent (hlist_hd (snd p)).
-          generalize dependent (hlist_tl (snd p)).
-          clear.
-          induction h0.
-          { reflexivity. }
-          { simpl. unfold hlist_get_cons_after_app in *. simpl.
-            eauto. } }
-        { intros. reflexivity. } }
-      { autorewrite with eq_rw in H2. forward; inv_all; subst.
-        replace (S (length tus)) with (length (tus ++ t :: nil)) in H0
-          by (rewrite app_length; simpl; omega).
-        rewrite substD_conv with (pfu := app_ass_trans tus (t :: nil) (map fst l))
-                                   (pfv := eq_refl) in H1.
-        autorewrite with eq_rw in H1. forward; inv_all; subst.
-        specialize (@IHl (tus ++ t :: nil) tvs _ _ _ _ H H0 H1 H2).
-        forward_reason.
-        rewrite substD_conv with (pfu := eq_sym (app_ass_trans tus (t :: nil) (map fst l)))
-                                   (pfv := eq_refl) in H3.
-        autorewrite with eq_rw in H3.
-        forward; inv_all; simpl in *; subst.
-        eexists; split; eauto.
-        intros.
-        autorewrite with eq_rw.
-        etransitivity; [ eapply H4 | clear H4 ].
-        autorewrite with eq_rw. reflexivity. } }
-  Qed.
-*)
 
   Lemma map_fst_combine : forall {T U} (ts : list T) (us : list U),
                             length ts = length us ->
@@ -206,73 +52,6 @@ Section runOnGoals.
     congruence. f_equal. auto.
   Qed.
 
-(*
-  Lemma forgets_length : forall z y x,
-                           length y = length (forgets x y z).
-  Proof.
-    induction y; simpl; auto.
-  Qed.
-
-  Lemma forgets_spec
-  (** TODO: There needs to be an extra requirement here that says that
-   ** the domain of s is in some way related to the range.
-   **)
-  : forall tvs ts tus s sD,
-      WellFormed_subst s ->
-      substD (tus ++ ts) tvs s = Some sD ->
-      exists s'D,
-        goal_substD tus tvs ts (forgets (length tus) ts s) = Some s'D /\
-        forall us vs,
-          s'D us vs <-> sD us vs.
-  Proof.
-(*
-    induction ts; simpl; intros.
-    { admit. (* eexists; split; eauto. simpl; auto. *) }
-    { consider (lookup (length tus) s); intros.
-      { admit. (*eapply substD_lookup in H1; eauto.
-                forward_reason.
-                assert (x = a) by admit.
-                subst.
-                rewrite substD_conv with (pfu := app_ass_trans tus (a :: nil) ts)
-                                         (pfv := eq_refl) in H0.
-                autorewrite with eq_rw in H0.
-                forward; inv_all; subst.
-                specialize (IHts (tus ++ a :: nil) s _ H H0).
-                forward_reason.
-                rewrite app_length in H4. simpl in H4.
-                rewrite Plus.plus_comm in H4.
-                simpl in H4.
-                rewrite H4.
-                eexists; split; eauto.
-                intros us vs H'; generalize (H3 us vs H'); clear H3.
-                autorewrite with eq_rw.
-                intros.
-                split.
-                { eapply H5. revert H'.
-                  autorewrite with eq_rw.
-                  clear.
-                  Lemma eq_sym_eq_sym : forall T (x y : T) (pf : x = y),
-                                          eq_sym (eq_sym pf) = pf.
-                  Proof.
-                    clear. destruct pf. reflexivity.
-                  Qed.
-                  rewrite eq_sym_eq_sym.
-                  tauto. }
-                { unfold hlist_get_cons_after_app.
-                  rewrite <- H3. revert H1. clear. intro.
-                  induction tus; simpl.
-                  { simpl in *. inv_all; subst.
-                    unfold hlist_nth. rewrite (hlist_eta us); simpl.
-                    rewrite <- (hlist_eta us).
-                    rewrite H.
-                    clear. autorewrite with eq_rw.
-                    admit. (** UIP: There should be a more natural phrasing **) }
-                  { admit. } } *) }
-      { admit. } }
-*)
-  Admitted.
-*)
-
   Lemma eta_ctx_subst_exs c ts (s : ctx_subst (CExs c ts))
   : exists y z,
       s = ExsSubst (typ:=typ) (expr:=expr) z y.
@@ -289,24 +68,6 @@ Section runOnGoals.
             end).
     eauto.
   Qed.
-(*
-  Instance Injective_WellFormed_ctx_subst_ExsSubst ctx ts c s
-  : Injective (WellFormed_ctx_subst (c:=CExs ctx ts) (ExsSubst c s)) :=
-    { result := WellFormed_ctx_subst c /\ WellFormed_subst s }.
-  intro.
-  refine match H in @WellFormed_ctx_subst _ _ _ _ _ _ _ C S
-               return match C as C return ctx_subst subst C -> Prop with
-                        | CExs _ _ => fun s' =>
-                                        let (s,c) := fromExs s' in
-                                        WellFormed_ctx_subst c /\ WellFormed_subst s
-                        | _ => fun _ => True
-                      end S
-         with
-           | WF_ExsSubst t c s s' pfs' pfs => conj  pfs pfs'
-           | _ => I
-         end.
-  Defined.
-*)
 
   Variable tac : rtac typ expr.
 
@@ -425,26 +186,7 @@ Section runOnGoals.
         end
     end.
 
-  Variables tus tvs : tenv typ.
-  Hypothesis Htac : rtac_sound tus tvs tac.
-
-(*
-  Lemma WellFormed_remembers
-  : forall b a s s',
-      remembers a b s = Some s' ->
-      WellFormed_subst s ->
-      WellFormed_subst s'.
-  Proof.
-    induction b; simpl; intros.
-    { inv_all; subst; auto. }
-    { forward. subst.
-      destruct o; forward.
-      { eapply IHb. eauto.
-        eapply set_sound in H1; eauto.
-        destruct H1; assumption. }
-      { eauto. } }
-  Qed.
-*)
+  Hypothesis Htac : rtac_sound tac.
 
   Local Hint Constructors WellFormed_ctx_subst.
   Lemma WellFormed_ctx_subst_fromAll
@@ -481,19 +223,6 @@ Section runOnGoals.
   Qed.
   Local Hint Resolve WellFormed_ctx_subst_fromAll WellFormed_ctx_subst_fromHyp.
 
-  Instance Injective_ExsSubst ts ctx a b c d
-  : Injective (ExsSubst (typ:=typ)(expr:=expr)(ts:=ts)(c:=ctx) a b = ExsSubst c d) :=
-    { result := a = c /\ b = d }.
-  intro pf.
-  refine (match pf in _ = X return
-                match X with
-                  | ExsSubst _ _ c d => fun a b => a = c /\ b = d
-                  | _ => True
-                end a b
-          with
-            | eq_refl => conj eq_refl eq_refl
-          end).
-  Defined.
 
 (*
   Lemma runOnGoals_list_sound_ind
@@ -509,24 +238,15 @@ Section runOnGoals.
                                    ctx s g).
 *)
 
-  Global Instance Injective_WellFormed_Goal_GAll tus tvs t g
-  : Injective (WellFormed_Goal tus tvs (GAll t g)) :=
-    { result := WellFormed_Goal tus (tvs ++ t :: nil) g }.
-  Proof. inversion 1; auto. Defined.
-  Global Instance Injective_WellFormed_Goal_GHyp tus tvs t g
-  : Injective (WellFormed_Goal tus tvs (GHyp t g)) :=
-    { result := WellFormed_Goal tus tvs g }.
-  Proof. inversion 1; auto. Defined.
-
 
   Lemma runOnGoals_sound_ind
   : forall g ctx s,
       @rtac_spec typ expr _ _ _
-                 tus tvs ctx s g
-                 (@runOnGoals (tus ++ getUVars ctx)
-                              (tvs ++ getVars ctx)
-                              (length tus + countUVars ctx)
-                              (length tvs + countVars ctx)
+                 ctx s g
+                 (@runOnGoals (getUVars ctx)
+                              (getVars ctx)
+                              (countUVars ctx)
+                              (countVars ctx)
                               ctx s g).
   Proof.
     red. induction g; fold runOnGoals in *.
@@ -538,22 +258,19 @@ Section runOnGoals.
         | H : match ?X with _ => _ end |- match match ?Y with _ => _ end with _ => _ end =>
           replace Y with X
       end; [ | f_equal ; try solve [ rewrite app_ass_trans ; reflexivity | omega ] ].
-      destruct (runOnGoals (tus ++ getUVars ctx) (tvs ++ getVars ctx ++ t :: nil)
-                           (length tus + countUVars ctx) (length tvs + S (countVars ctx))
+      destruct (runOnGoals (getUVars ctx) (getVars ctx ++ t :: nil)
+                           (countUVars ctx) (S (countVars ctx))
                            (AllSubst s) g);
         auto; intros; forward_reason; inv_all.
       { destruct IHg as [ ? [ ? ? ] ].
-        { rewrite app_assoc. assumption. }
+        { assumption. }
         { constructor. auto. }
         split.
         { apply WellFormed_ctx_subst_fromAll; auto. }
         split.
-        { constructor. rewrite <- app_assoc; eauto. }
-        { generalize (Proper_pctxD_impl tus tvs (fromAll c)).
+        { constructor. eauto. }
+        { generalize (Proper_pctxD_impl (fromAll c)).
           simpl in *.
-          rewrite goalD_conv with (pfu := eq_refl)
-                                    (pfv := eq_sym (app_ass_trans tvs (getVars ctx) (t :: nil))).
-          autorewrite with eq_rw.
           forward; inv_all; subst.
           forward_reason.
           inv_all; subst; simpl in *.
@@ -563,7 +280,6 @@ Section runOnGoals.
           eapply H6; [ | reflexivity | reflexivity | eapply H9 ].
           do 6 red. clear.
           do 6 intro; equivs.
-          destruct (app_ass_trans tvs (getVars ctx) (t :: nil)); simpl.
           eauto. } }
       { admit. (* generalize (Proper_pctxD_impl tus tvs (fromAll c)).
         simpl in *.
@@ -584,135 +300,85 @@ Section runOnGoals.
     { (* Exs *)
       intros; simpl in *.
       forward.
-      specialize (@IHg (CExs _ l) (ExsSubst s r)).
+      specialize (@IHg (CExs _ l) (ExsSubst s a)).
       revert IHg.
       repeat rewrite countUVars_getUVars.
       repeat rewrite countVars_getVars.
-      do 2 rewrite <- app_length.
       intros; forward.
       match goal with
         | H : match ?X with _ => _ end |- match match ?Y with _ => _ end with _ => _ end =>
           replace Y with X;
             [ remember X as X' ; destruct X'
-            |  ]
+            | simpl; f_equal; rewrite app_length; omega ]
       end; intros; auto.
       { destruct (eta_ctx_subst_exs c) as [ ? [ ? ? ] ]; subst.
         simpl. intros.
         destruct IHg as [ ? [ ? ? ] ].
-        { inversion H; subst; auto. simpl in *.
-          rewrite app_assoc. assumption. }
+        { inversion H; subst; auto. }
         { inversion H; subst. constructor; auto.
-          
-        generalize (WellFormed_remembers _ _ _ H (@WellFormed_empty _ _ _ _ _ _ _ _ _)); intros.
-        forward_reason.
-        inv_all; split; auto.
-        simpl in *. forward; inv_all; subst.
-        destruct (substD_empty ((tus ++ getUVars ctx) ++ map fst l) (tvs ++ getVars ctx)) as [ ? [ ? ? ] ].
-        destruct (@remembers_spec _ _ _ _ _ _ _ (@WellFormed_empty _ _ _ _ _ _ _ _ _) H H10 H9) as [ ? [ ? ? ] ].
-        rewrite H12 in H8.
-        forward; inv_all; subst.
-        rewrite map_fst_combine in * by eauto using forgets_length.
-        rewrite map_snd_combine in * by eauto using forgets_length.
-        Cases.rewrite_all_goal.
-        eapply forgets_spec in H8; eauto.
-        destruct H8 as [ ? [ ? ? ] ].
-        Cases.rewrite_all_goal.
-        forward_reason.
-        inv_all. subst.
-        split; auto.
-        { intros us vs.
-          specialize (H18 us vs); revert H18.
-          rewrite H12 in H15. rewrite H16 in *.
-          rewrite H1 in *.
-          forwardy.
-          eapply forgets_spec in H15; eauto.
-          specialize (H18 us vs).
-          eapply Ap_pctxD; eauto.
-          revert H18.
-          eapply Ap_pctxD; eauto.
-          eapply Pure_pctxD; eauto.
+          rewrite countUVars_getUVars. assumption. }
+        simpl in *.
+        forward.
+        inv_all.
+        inv_all.
+        split; auto. split.
+        { constructor; eauto.
+          rewrite countUVars_getUVars in H8. assumption. }
+        { forward. inv_all. subst.
+          forward_reason. inv_all; subst.
+          revert H12.
+          Cases.rewrite_all_goal. intros.
+          split; auto. reflexivity.
           intros.
-          forward_reason.
-          rewrite H8 in H15. inv_all. subst.
-          clear - H11 H13 H17 H18 H19 H20 H22.
-          rewrite _forall_sem in H19.
-          rewrite _exists_sem in H20.
-          destruct H20.
-          apply _exists_sem. exists x0.
-          specialize (H11 (hlist_app us0 x0) vs0).
-          specialize (H13 (hlist_app us0 x0) vs0).
-          destruct H.
-          split.
-          { destruct H13. destruct H2; eauto.
-            eapply H18. eapply H22. assumption. }
-          { eapply H19; auto. apply H17. auto. } } }
-      { (** Same Proof as above **)
-        destruct (eta_ctx_subst_exs c) as [ ? [ ? ? ] ]; subst.
+          generalize (H14 us vs); clear H14.
+          eapply Ap_pctxD; eauto.
+          generalize (H12 us vs); clear H12.
+          eapply Fmap_pctxD_impl; eauto; try reflexivity.
+          clear.
+          do 6 red; intros.
+          eapply _exists_sem.
+          eapply _exists_sem in H3. destruct H3.
+          exists x1.
+          rewrite _forall_sem in H2.
+          equivs. firstorder. } }
+      { destruct (eta_ctx_subst_exs c) as [ ? [ ? ? ] ]; subst.
         simpl. intros.
-        generalize (WellFormed_remembers _ _ _ H (@WellFormed_empty _ _ _ _ _ _ _ _ _)); intros.
-        forward_reason.
-        inv_all; split; auto.
-        simpl in *. forward; inv_all; subst.
-        destruct (substD_empty ((tus ++ getUVars ctx) ++ map fst l) (tvs ++ getVars ctx)) as [ ? [ ? ? ] ].
-        destruct (@remembers_spec _ _ _ _ _ _ _ (@WellFormed_empty _ _ _ _ _ _ _ _ _) H H10 H9) as [ ? [ ? ? ] ].
-        rewrite H12 in H8.
-        forward; inv_all; subst.
-        rewrite map_fst_combine in * by eauto using forgets_length.
-        rewrite map_snd_combine in * by eauto using forgets_length.
-        Cases.rewrite_all_goal.
-        eapply forgets_spec in H8; eauto.
-        destruct H8 as [ ? [ ? ? ] ].
-        Cases.rewrite_all_goal.
-        forward_reason.
-        inv_all. subst.
+        inv_all.
+        destruct IHg as [ ? ? ]; eauto.
+        { constructor; eauto. rewrite countUVars_getUVars. assumption. }
+        inv_all.
+        split; auto. split.
+        { constructor; auto. rewrite <- countUVars_getUVars. assumption.
+          constructor. }
+        simpl in *.
+        forward. inv_all; subst.
+        forward_reason. inv_all; subst.
         split; auto.
-        { intros us vs.
-          specialize (H17 us vs); revert H17.
-          repeat match goal with
-                   | H : _ = _ , H' : _ |- _ =>
-                     rewrite H in H'
-                 end.
-          forwardy.
-          eapply forgets_spec in H14; eauto.
-          specialize (H17 us vs).
-          eapply Ap_pctxD; eauto.
-          revert H17.
-          eapply Ap_pctxD; eauto.
-          eapply Pure_pctxD; eauto.
-          intros.
-          forward_reason.
-          rewrite H8 in H14. inv_all. subst.
-          clear - H21 H17 H18 H16 H19 H13.
-          rewrite _forall_sem in H18.
-          rewrite _exists_sem in H19.
-          destruct H19.
-          apply _exists_sem. exists x0.
-          specialize (H16 (hlist_app us0 x0) vs0).
-          specialize (H21 (hlist_app us0 x0) vs0).
-          specialize (H13 (hlist_app us0 x0) vs0).
-          destruct H.
-          split.
-          { destruct H13. destruct H2; eauto.
-            eapply H17. eapply H21. assumption. }
-          { eapply H18; auto. apply H16. auto. } } }  *)}
+        intros.
+        revert H10.
+        Cases.rewrite_all_goal. intros.
+        generalize (H10 us vs); clear H10.
+        eapply Ap_pctxD; eauto.
+        generalize (H12 us vs); clear H12.
+        eapply Fmap_pctxD_impl; eauto; try reflexivity.
+        clear.
+        do 6 red. intros.
+        eapply _exists_sem.
+        eapply _exists_sem in H3. destruct H3.
+        exists x1.
+        rewrite _forall_sem in H1.
+        equivs. firstorder. } }
     { (* Hyp *)
       simpl; intros.
       specialize (IHg (CHyp ctx e) (HypSubst s)).
+      simpl in *.
       match goal with
         | H : match ?X with _ => _ end
           |- match match ?Y with _ => _ end with _ => _ end =>
           replace Y with X; [ remember X as X' ; destruct X' | f_equal ; simpl ; rewrite map_length; omega ]
-      end; auto;
-      intros; forward_reason; split; eauto; simpl in *;
-      forward; forward_reason; subst; inv_all; subst; simpl in *;
-      forward; subst; inv_all; subst.
-      { split; auto.
-        intros us vs.
-        generalize (H7 us vs).
-        eapply Fmap_pctxD_impl; try reflexivity; eauto.
-        clear; do 6 red; intros.
-        equivs; tauto. }
-      { split; auto. } }
+      end; auto.
+      { admit. }
+      { admit. } }
     { (* Conj *)
       simpl; intros; clear Htac.
       specialize (IHg1 ctx s).
@@ -730,40 +396,42 @@ Section runOnGoals.
             |- context [ match ?Y with _ => _ end ] =>
             change Y with X ; destruct X; auto
         end.
-        { rename g into B'.
-          intros; forward_reason; split; auto.
+        { 
+          Global Instance Injective_WellFormed_Goal_GConj tus tvs a b
+          : Injective (WellFormed_Goal tus tvs (GConj_ a b)) :=
+          { result := WellFormed_Goal tus tvs a /\ WellFormed_Goal tus tvs b }.
+          Proof. inversion 1. auto. Defined.
+          intros; inv_all.
+          forward_reason.
+          split; auto.
+          split; [ constructor; auto | ].
           simpl. forward. forward_reason.
-          split; [ etransitivity; eassumption | ].
+          split; [ etransitivity; eauto | ].
           intros us vs.
-          specialize (H11 us vs).
-          specialize (H12 us vs).
-          revert H11.
-          eapply (Applicative_pctxD _ H8).
-          eapply pctxD_SubstMorphism.
-          3: eassumption. eassumption. eassumption.
-          revert H12.
-          eapply (Fmap_pctxD_impl _ H3); try reflexivity.
+          generalize (H15 us vs); clear H15.
+          eapply Ap_pctxD; eauto.
+          eapply pctxD_SubstMorphism; eauto.
+          generalize (H16 us vs); clear H16.
+          eapply Fmap_pctxD_impl; eauto; try reflexivity.
           clear. do 6 red.
           intros. equivs. firstorder. }
-        { change (rtac_spec tus tvs s (GConj_ A B) (More c0 A')).
+        { change (rtac_spec s (GConj_ A B) (More c0 A')).
           eapply Proper_rtac_spec; [ reflexivity | eapply More_More_ | ].
           reflexivity.
           simpl.
-          intros; forward_reason; split; auto.
-          simpl. forward. forward_reason.
+          intros; inv_all; forward_reason.
+          split; auto. split; auto.
+          forward. forward_reason.
           split; [ etransitivity; eassumption | ].
           intros us vs.
-          specialize (H11 us vs).
-          specialize (H10 us vs).
-          revert H10.
-          eapply (Applicative_pctxD _ H8).
-          eapply pctxD_SubstMorphism.
-          3: eassumption. eassumption. eassumption.
-          revert H11.
-          eapply (Fmap_pctxD_impl _ H3); try reflexivity.
+          generalize (H13 us vs); clear H13.
+          eapply Ap_pctxD; eauto.
+          eapply pctxD_SubstMorphism; eauto.
+          generalize (H14 us vs); clear H14.
+          eapply Fmap_pctxD_impl; eauto; try reflexivity.
           clear. do 6 red.
           intros. equivs. firstorder. } }
-      { specialize (IHg2 ctx c).
+      { admit. (* specialize (IHg2 ctx c).
         match goal with
           | H : match ?X with _ => _ end
             |- context [ match ?Y with _ => _ end ] =>
@@ -797,52 +465,46 @@ Section runOnGoals.
           revert H10.
           eapply (Fmap_pctxD_impl _ H3); try reflexivity.
           clear. do 6 red.
-          intros. equivs. firstorder. } } }
+          intros. equivs. firstorder. } } *) } }
     { (* Goal *)
       clear - Htac; simpl; intros.
       red in Htac.
       specialize (@Htac ctx s e _ eq_refl).
       rewrite countUVars_getUVars.
       rewrite countVars_getVars.
-      do 2 rewrite <- app_length.
       eauto. }
     { (* Solved *)
       clear. simpl.
       intros. split; auto.
-      forward. split; [ reflexivity | ].
+      forward.
+      split; [ reflexivity | ].
       intros.
-      eapply (@Applicative_pctxD _ _ _ _ _ _ _ _ tus tvs ctx s); eauto. }
+      eapply Pure_pctxD; eauto. }
   Qed.
 
 End runOnGoals.
 
-Arguments runOnGoals {typ expr subst _ _} tac tus tvs nus nvs ctx csub goal : rename.
+Arguments runOnGoals {typ expr} tac tus tvs nus nvs ctx csub goal : rename.
 
 Section runOnGoals_proof.
   Variable typ : Type.
   Variable expr : Type.
-  Variable subst : Type.
 
   Context {RType_typ : RType typ}.
   Context {Expr_expr : Expr RType_typ expr}.
   Context {Typ0_Prop : Typ0 _ Prop}.
-  Context {Subst_subst : Subst subst expr}.
-  Context {SubstOk_subst : @SubstOk _ _ _ _ Expr_expr Subst_subst}.
-  Context {SubstUpdate_subst : SubstUpdate subst expr}.
-  Context {SubstUpdateOk_subst : @SubstUpdateOk _ _ _ _ Expr_expr Subst_subst _ _}.
 
   Theorem runOnGoals_sound
-  : forall tus tvs tac,
-      rtac_sound tus tvs tac -> rtacK_sound tus tvs (runOnGoals tac).
+  : forall tac,
+      rtac_sound tac -> rtacK_sound (runOnGoals tac).
   Proof.
     intros.
-    generalize (@runOnGoals_sound_ind typ expr subst _ _ _ _ _ _ tac tus tvs H).
+    generalize (@runOnGoals_sound_ind typ expr _ _ _ tac H).
     red. intros; subst.
     specialize (H0 g ctx s). revert H0; clear.
     unfold rtac_spec, rtacK_spec.
     rewrite countUVars_getUVars.
     rewrite countVars_getVars.
-    do 2 rewrite <- app_length.
     exact (fun x => x).
   Qed.
 End runOnGoals_proof.
